coq/Completeness.v
@@ -312,6 +312,28 @@ Proof.
       }
       {
         inversion H4; subst.
+        destruct t1; try apply OA_None.
+        destruct t2;
+        try (
+          simpl;
+          repeat (destruct w; try apply OA_None);
+          destruct (make_dynamic_int sort (smt_eval_ast m sort ast)); apply OA_None
+        ).
+        {
+          rename w into w1, w0 into w2.
+          repeat (destruct w1; try apply OA_None);
+          (
+            simpl;
+            destruct sort; try apply OA_None;
+            repeat (destruct w2; try apply OA_None);
+            simpl;
+            eapply OA_Some;
+            [ reflexivity | reflexivity ]
+          ).
+        }
+      }
+      {
+        inversion H4; subst.
         destruct t1, t2;
         try apply OA_None.
         simpl.
