coq/DynamicValue.v
@@ -198,17 +198,23 @@ Definition convert conv x t1 t2 : option dynamic_value :=
   | Zext =>
       match t1, x, t2 with
       | TYPE_I 8, DV_Int (DI_I8 i1), TYPE_I 32 =>
-        Some (DV_Int (DI_I32 (repr (unsigned i1))))
+          Some (DV_Int (DI_I32 (repr (unsigned i1))))
       | TYPE_I 32, DV_Int (DI_I32 i1), TYPE_I 64 =>
-        Some (DV_Int (DI_I64 (repr (unsigned i1))))
+          Some (DV_Int (DI_I64 (repr (unsigned i1))))
       | _, _, _ => None
       end
   | Sext =>
       match t1, x, t2 with
       | TYPE_I 8, DV_Int (DI_I8 i1), TYPE_I 32 =>
-        Some (DV_Int (DI_I32 (repr (signed i1))))
+          Some (DV_Int (DI_I32 (repr (signed i1))))
       | TYPE_I 32, DV_Int (DI_I32 i1), TYPE_I 64 =>
-        Some (DV_Int (DI_I64 (repr (signed i1))))
+          Some (DV_Int (DI_I64 (repr (signed i1))))
+      | _, _, _ => None
+      end
+  | Trunc =>
+      match t1, x, t2 with
+      | TYPE_I 32, DV_Int (DI_I32 i1), TYPE_I 8 =>
+          Some (DV_Int (DI_I8 (repr (unsigned i1))))
       | _, _, _ => None
       end
   | Bitcast =>
@@ -217,6 +223,5 @@ Definition convert conv x t1 t2 : option dynamic_value :=
           if (bits1 =? bits2)%positive then Some x else None
       | _, _, _ => None
       end
-  | _ => None
   end
 .
