coq/ExecutionTreeOpt.v
@@ -297,6 +297,20 @@ Proof.
         inversion Heval; subst;
         eexists;
         split;
+        [ reflexivity | apply equiv_smt_expr_extract; assumption ]
+      ).
+    }
+    {
+      destruct t1; try discriminate Heval.
+      destruct t2; try discriminate Heval.
+      rename w into w1, w0 into w2.
+      repeat (destruct w1; try discriminate Heval);
+      (
+        destruct sort'; try discriminate Heval;
+        repeat (destruct w2; try discriminate Heval);
+        inversion Heval; subst;
+        eexists;
+        split;
         [ reflexivity | apply equiv_smt_expr_zext; assumption ]
       ).
     }
